Iterator class like in VST/progs/verif_message.v

verif/db/verif_operations.v
@@ -1,13 +1,16 @@
 Require Import VST.floyd.proofauto.
-
 Require Import Signatures.
-
 Require Import db_operations.
+
+Require btrees.btrees. Require btrees.btrees_sep. 
+
 
 Instance CompSpecs : compspecs. make_compspecs prog. Defined.
 Definition Vprog : varspecs. mk_varspecs prog. Defined.
 
 Require Import FiniteSet FlatData SortedTuples SortedAttributes Values Plans.
+
+Require SeqScan.
 
 Fixpoint string_to_list_byte (s: string) : list byte :=
   match s with
@@ -35,14 +38,12 @@ Definition tuple_rep (sh : share) (t : tuple) (p : val) : mpred :=
           data_at sh (tarray size_t (Z.of_nat (Fset.cardinal FAN (support t))))
                   (map (val_of_value sp oo dot t) (Fset.elements FAN (support t))) p * stringpool_rep sp.
 
-Definition t_attr_list := Tstruct _attribute_list_t noattr.
+Definition t_attr_list_t := Tstruct _attribute_list_t noattr.
 
 Definition id_of_attribute (a : attribute) : list byte :=
   match a with
   | Attr_string _ s => string_to_list_byte s
   | Attr_ptrofs _ s => string_to_list_byte s end.
-
-Eval compute in reptype t_attr_list.
 
 Definition domain_of_attribute (a : attribute) : val :=
   match a with
@@ -58,7 +59,7 @@ Fixpoint attribute_lseg_rep (sh : share) (l : list attribute) (p q : val) : mpre
   match l with
   | [] => !! (p = q /\ is_pointer_or_null p) && emp
   | a :: tl =>
-    EX r : val, EX sptr : val, data_at sh t_attr_list (sptr, (domain_of_attribute a, r)) p * attribute_lseg_rep sh tl r q * attribute_string_rep sh a sptr end.
+    EX r : val, EX sptr : val, data_at sh t_attr_list_t (sptr, (domain_of_attribute a, r)) p * attribute_lseg_rep sh tl r q * attribute_string_rep sh a sptr end.
 
 Lemma attribute_lseg_nil sh l : attribute_lseg_rep sh l nullval nullval |-- !! (l = []).
 Proof.
@@ -112,8 +113,8 @@ Definition attributes_rep (sh : share) (attrs : Fset.set FAN) (p : val) : mpred 
 
 Definition attribute_list_length_spec :=
  DECLARE _attribute_list_length
-  WITH sh : share, l: val, attrs: Fset.set FAN
-  PRE [ _l OF (tptr t_attr_list)]
+  WITH sh: share, l: val, attrs: Fset.set FAN
+  PRE [ _l OF (tptr t_attr_list_t)]
      PROP(readable_share sh)
      LOCAL (temp _l l; temp _x l)
      SEP (attributes_rep sh attrs l)
@@ -122,8 +123,86 @@ Definition attribute_list_length_spec :=
      LOCAL(temp ret_temp (Vint (Int.repr (Z.of_nat (Fset.cardinal _ attrs)))))
      SEP (attributes_rep sh attrs l).
 
-Definition Gprog := ltac:(with_library prog [attribute_list_length_spec]).
-Print Fset.
+Import QEP. (* QEP.cursor --> cursor *)
+
+Definition t_iterator_t := Tstruct _iterator_t noattr.
+Definition t_methods := Tstruct _methods noattr.
+Definition t_seq_scan_env := Tstruct _seq_scan_env noattr.
+Definition t_index_join_env := Tstruct _index_join_env noattr.
+
+Local Notation O := (Tuple.OTuple TPL.T).
+
+Record iterator_class (c: Cursor.Rcd O) :=
+  {
+    env: Type;
+    env_rep: env -> val -> mpred;
+    env_init: env -> env;
+    env_next: env -> env;
+    (* axioms *)
+    env_close: env -> env;
+  }.
+Arguments env {c}.
+Arguments env_init {c}.
+Arguments env_next {c}.
+Arguments env_close {c}.
+Arguments env_rep {c}.
+
+Definition result_rep sh (r : result tuple) (p: val) : mpred :=
+  match r with
+  | Result t => tuple_rep sh t p
+  | No_Result => emp (* ??? *)
+  | Empty_Cursor => !! (p = nullval) end.
+
+Definition next_spec {c: Cursor.Rcd O} (cl : iterator_class c) :=
+  WITH p: val, e: env cl, it: Cursor.cursor c, t: val, sh: share
+  PRE [ _env OF (tptr tvoid) ]
+  PROP()
+  LOCAL(temp _env p)
+  SEP(env_rep cl e p)
+  POST [ tptr tvoid ]
+  PROP()
+  LOCAL(temp ret_temp t)
+  SEP(result_rep sh (fst (Cursor.next it)) t * cl.(env_rep) (cl.(env_next) e) p).
+
+Definition seqscan_iterator : iterator_class (SeqScan.SeqScan.build O) :=
+  {|
+    env := btrees.relation val * btrees.cursor val;
+    env_rep := fun e p =>
+                 let (rel, cur) := e in
+                 let (relnode, qrel) := rel in
+                 EX qcur: val,
+                                        data_at Tsh t_seq_scan_env (qrel, qcur) p *
+                                        btrees_sep.relation_rep (fst e) (btrees.get_numrec (fst e)) *
+                                        btrees_sep.cursor_rep (snd e) (fst e) qcur;
+    env_init := fun e => (fst e, btrees.moveToFirst (fst (fst e)) (snd e) 0);
+    env_next := fun e => (fst e, btrees.moveToNext (snd e) (fst e));
+    env_close := fun e => e; (* FreeRecord? *)
+  |}.
+
+Definition seqscan_next_spec := (DECLARE _seq_scan_next (next_spec seqscan_iterator)).
+
+(* MATERIALIZE: WORK IN PROGRESS
+Definition materialize_spec :=
+  DECLARE _materialize
+    WITH sh: share, a: val, it: val, c: cursor
+    PRE [ _it OF (tptr t_iterator_t) ]
+    PROP()
+    LOCAL(temp _it it; temp _a a)
+    SEP(iterator_rep sh c it)
+    POST [  *)
+
+Definition Gprog := ltac:(with_library prog [attribute_list_length_spec; seqscan_next_spec]).
+
+Lemma body_seqscan_next: semax_body Vprog Gprog f_seq_scan_next seqscan_next_spec.
+Proof.
+  unfold seqscan_next_spec, next_spec.
+  start_function.
+  simpl env_rep.
+  destruct e as [rel c], rel as [relnode qrel].
+  Intros qcur.
+  forward.
+Admitted.  
+
 Lemma body_attribute_list_length: semax_body Vprog Gprog f_attribute_list_length attribute_list_length_spec.
 Proof.
   start_function.
@@ -154,3 +233,4 @@ Proof.
     rewrite Fset.cardinal_spec. rewrite Zlength_correct; auto. entailer!.
     unfold attributes_rep, attribute_list_rep. sep_apply attribute_lseg_nil. simpl. entailer!.
 Qed.
+
